tc works

CryptoPrims/CryptoTests.lean
@@ -1,14 +1,194 @@
 import Lean
 import OwlLean.TypeChecker.OwlComplete
-import OwlLean.TypeChecker.TcSimple
 
 open Lean Meta Elab Tactic
 
-open OwlTypecheck
+open OwlTc
 
+/-
+@[simp]
+def Sequent.ok (s : Sequent) :=
+  OwlTc.has_type_infer s.Phi s.Psi s.Delta s.Gamma s.e s.t
+-/
+
+
+elab "whnf" : tactic => do
+  -- 1. Get the current main goal
+  let goal ← getMainGoal
+
+  -- 2. Use goal.withContext to ensure we can see local variables
+  goal.withContext do
+    let reduced ← whnf (<- goal.getType)
+    let newGoal ← goal.change reduced
+    replaceMainGoal [newGoal]
+
+elab "done" : tactic => do
+  -- 1. Get the current main goal
+  let goal ← getMainGoal
+  match <- goal.getType with
+  | .app (.app (.const `OwlTc.TypeError _) stx) e => do
+    let s <- unsafe evalExpr String (mkConst ``String) e
+    let stx' <- unsafe evalExpr (Option Owl.opaqueSyntax)
+      (mkApp (mkConst ``Option [.zero]) (mkConst ``Owl.opaqueSyntax []))
+      stx
+    let newGoal := Expr.app (.app (.const `OwlTc.TypeError []) stx) (mkStrLit s)
+    let newGoal <- goal.change newGoal
+    replaceMainGoal [newGoal]
+    match stx' with
+    | some v =>
+      logInfo "got syntax"
+      logErrorAt v.inner s
+    | _ => pure ()
+    logInfo s
+  | _ => pure ()
+
+
+
+attribute [simp] Fin.foldr_succ
+
+def encI :=
+( · ; · ; · ; · ⊢
+    Λβ betaK .
+    Λβ betaM .
+    Λ tau .
+    let k = (⟨"genKey"⟩ (["0"], ["0"]) : Data betaK) in
+    let L = alloc (λ (null : Public) : (tau + unit) => ı2 *) in
+    let enc' = (corr_case betaK in
+                (if corr ( betaK )
+                  then (λ (x : (Public * Public)) : Public => ⟨"enc"⟩ (π1 x, π2 x))
+                  else
+                    λ (x : (Data betaK * tau)) : Public =>
+                    let c = ⟨"rand"⟩ (zero ((π2 x) : Data betaM), ["0"]) in
+                    let L_old = (! L) in
+                    let sc = (L := (λ (y : Public) : (tau + unit) => if ⟨"eq"⟩(y, c) then ı1 (π2 x) else (L_old [y]))) in
+                    c))
+    in
+    let dec' : corr (betaK) ? (Public * Public) -> Public : (Data betaK * Public) -> (tau + unit) = (corr_case betaK in
+               (if corr (betaK) then λ (x : (Public * Public)) : Public => ⟨"dec"⟩(π1 x, π2 x)
+                else λ (x : (Data betaK * Public)) : (tau + unit) => (!L) [π2 x]))
+    in
+    pack (Data betaK, ⟨k, ⟨(corr_case betaK in enc'), dec'⟩⟩)
+    :
+    ∀ betaK ⊒ ⟨Owl.L.bot⟩ .
+    ∀ betaM ⊏ betaK .
+    ∀ tau <: Data betaM .
+    (∃ alphaK <: (Data betaK) . (alphaK *
+                                 ((corr (betaK) ? (Public * Public) -> Public : (alphaK * tau) -> Public) *
+                                  (corr (betaK) ? (Public * Public) -> Public : (alphaK * Public) -> (tau + unit))))))
+
+
+
+
+
+#check Command.CommandElabM
+
+
+def addTypeInfo (stx : Syntax) (s : String) := do
+    let n : Name := Name.mkSimple s
+
+    withEnableInfoTree true do withLocalDeclD n (mkSort levelOne) fun dslType => do
+      let forgedExpr ← mkFreshExprMVar dslType
+      pushInfoLeaf <| .ofTermInfo {
+        elaborator := `Sequent
+        stx := stx
+        lctx := (← getLCtx)
+        expectedType? := some dslType
+        expr := forgedExpr
+        isBinder := false
+      }
+    pure ()
+
+def tcVisit l d (o : Owl.opaqueSyntax) (t : Owl.ty l d) : Command.CommandElabM Unit  := do
+  Command.liftTermElabM $ addTypeInfo o.inner (toString t)
+  pure ()
+
+def tcLog (s : String) : Command.CommandElabM Unit := do
+  -- Command.liftTermElabM $ logInfo s
+  IO.println s
+  pure ()
+
+syntax "#tc" term "by" tacticSeq : command
+
+@[simp]
+def interpSideConditions (ls : List SideCondition) : Prop :=
+  List.foldr (fun i acc => i.interp ∧ acc) True ls
+
+def mkFreshDefn (e : Expr) : Command.CommandElabM Ident := do
+  let lctx ← Command.liftTermElabM $ getLCtx
+  let name := LocalContext.getUnusedName lctx `freshDef
+  let id := mkIdent name
+  Command.liftTermElabM <| do
+    -- add definition: freshDef := e
+    Lean.addDecl <| .defnDecl {
+      name := name,
+      levelParams := [],
+      type := ← inferType e,
+      value := e,
+      hints := .abbrev,
+      safety := DefinitionSafety.safe
+    }
+  pure id
+
+elab_rules : command
+  | `(#tc $e by%$tkp $pf:tacticSeq ) => do
+    let s ← Command.liftTermElabM $ Lean.Elab.Term.elabTerm e (.some (.const `Sequent []))
+    let s <- Command.liftTermElabM $ unsafe evalExpr Sequent (mkConst `Sequent) s
+    match <- OwlTc.infer s.Phi s.Psi s.Delta s.Gamma s.e s.t (CheckState.init tcVisit tcLog) with
+    | .ok (_, p) => do
+      let sc := p.side_condition
+      let id <- mkFreshDefn (toExpr sc)
+      let lemmaName <- (Command.liftTermElabM $ mkFreshUserName `_)
+      let thmCmd <- withRef tkp `(command|
+        theorem $(mkIdent lemmaName) : interpSideConditions $id := by $pf
+      )
+      Command.elabCommand thmCmd
+    | .err e =>
+      logInfo s!"err: {e.2}"
+      match e.1 with
+      | .none => pure ()
+      | .some v =>
+        logErrorAt v.inner e.2
+    -- Alternatively, use macros or custom translation if Sequent is not a constructor
+    -- let s : Sequent := ... -- adjust as needed depending on the definition of Sequent
+
+
+#tc encI by {
+    unfold freshDef
+    simp
+    grind
+}
+
+
+syntax "#tst" "by" tacticSeq : command
+
+elab_rules : command
+  | `(#tst by%$tkp $pf:tacticSeq) => do
+
+    let lemmaName <- (Command.liftTermElabM $ mkFreshUserName `_)
+
+    let thmCmd <- withRef tkp `(command|
+      theorem $(mkIdent lemmaName) : True := by $pf
+    )
+    Command.elabCommand thmCmd
+
+#tst by {
+    sorry
+}
+
+#check
+
+
+
+
+
+
+
+
+
+
+/-
 
 -- "[0]" represents garbage values not needed for computation
-/-
 theorem enc_i :
   ( · ; · ; · ; · ⊢
     Λβ betaK .
@@ -37,19 +217,42 @@ theorem enc_i :
     ∀ tau <: Data betaM .
     (∃ alphaK <: (Data betaK) . (alphaK *
                                  ((corr (betaK) ? (Public * Public) -> Public : (alphaK * tau) -> Public) *
-                                  (corr (betaK) ? (Public * Public) -> Public : (alphaK * Public) -> (tau + Unit)))))) :=
+                                  (corr (betaK) ? (Public * Public) -> Public : (alphaK * Public) -> (tau + Unit)))))).ok :=
     by
-    apply OwlTypecheck.infer_sound
+      simp
+      whnf
+      simp
+      done
 
 
-    unfold OwlTypecheck.infer
 
 
 
 
-    rw [OwlTypecheck.infer]
 
--/
+
+
+
+
+
+
+
+
+
+
+      -- Public -> (x + Unit)
+      -- x + Unit
+
+
+
+
+
+
+
+
+
+
+
 
 /-
 
@@ -178,42 +381,13 @@ abbrev mySeq := ( (l1, l2 ⊒ l1, l3 ⊒ l2) ; · ; (a <: Data l2, b <: Data l1)
     :
     Public)
 
-@[inline]
-def Sequent.ok (s : Sequent) :=
-  OwlTc.has_type_infer s.Phi s.Psi s.Delta s.Gamma s.e s.t
 
-#reduce (types := true) mySeq.ok
-
-partial def unfoldAll (e : Expr) (declName : Name) : MetaM Expr := do
-  if let some unfolded ← unfoldDefinition? e (ignoreTransparency := true) then
-    unfoldAll unfolded declName
-  else
-    -- Fallback to standard reduction if it's no longer the head constant
-    reduce e
-
-elab "eval_goal" : tactic => do
-  -- 1. Get the current main goal
-  let goal ← getMainGoal
-
-  -- 2. Use goal.withContext to ensure we can see local variables
-  goal.withContext do
-    let type ← goal.getType
-
-    -- 3. Reduce the type (this is MetaM)
-    let reduced ← reduce (skipTypes := false) type
-
-    -- 4. Change the goal and get the new MVarId
-    let newGoal ← goal.change reduced
-
-    -- 5. Update the tactic state with the new goal
-    replaceMainGoal [newGoal]
-    evalTactic (<- `(tactic| simp))
-
-
-attribute [simp] Fin.foldr_succ
 
 
 theorem enc_layered :
   mySeq.ok :=  by
-    eval_goal;
+    whnf
+    simp
     grind
+
+-/
