OwlLean/OwlLang/ToString.lean
@@ -1,0 +1,62 @@
+import OwlLean.OwlLang.Owl
+
+namespace Owl
+
+def cond_sym.pretty (c : cond_sym) : String :=
+  match c with
+  | .leq   => "≤"
+  | .geq   => "≥"
+  | .gt    => ">"
+  | .lt    => "<"
+  | .nleq  => "≰"
+  | .ngeq  => "≱"
+  | .ngt   => "≯"
+  | .nlt   => "≮"
+
+instance : ToString cond_sym where
+  toString := cond_sym.pretty
+
+def label.pretty (l : label n) : String :=
+  match l with
+  | .var_label i => "L" ++ toString i.toNat
+  | .latl _ => "<lconst>"
+  | .ljoin l1 l2 => "(" ++ l1.pretty ++ " ⊔ " ++ l2.pretty ++ ")"
+  | .lmeet l1 l2 => "(" ++ l1.pretty ++ " ⊓ " ++ l2.pretty ++ ")"
+  | .default => "Ldefault"
+
+instance : ToString (label n) where
+  toString := label.pretty
+
+
+def binary.pretty (b : binary) : String :=
+  match b with
+  | .bend => "ε"
+  | .bzero b' => "0" ++ b'.pretty
+  | .bone b' => "1" ++ b'.pretty
+
+instance : ToString binary where
+  toString := binary.pretty
+
+
+def ty.pretty (t : ty l d) : String :=
+  match t with
+  | .var_ty i => "X" ++ toString i.toNat
+  | .Any => "Any"
+  | .Unit => "Unit"
+  | .Data l => "Data[" ++ l.pretty ++ "]"
+  | .Ref t' => "Ref(" ++ t'.pretty ++ ")"
+  | .arr t1 t2 => "(" ++ t1.pretty ++ " -> " ++ t2.pretty ++ ")"
+  | .prod t1 t2 => "(" ++ t1.pretty ++ " * " ++ t2.pretty ++ ")"
+  | .sum t1 t2 => "(" ++ t1.pretty ++ " + " ++ t2.pretty ++ ")"
+  | .all t0 t => "forall (" ++ t0.pretty ++ "), " ++ t.pretty
+  | .ex t0 t => "exists (" ++ t0.pretty ++ "), " ++ t.pretty
+  | .all_l cs l t =>
+      "forall(" ++ cs.pretty ++ " " ++ l.pretty ++ "). " ++ t.pretty
+  | .t_if l t1 t2 =>
+      "if[" ++ l.pretty ++ "] { " ++ t1.pretty ++ " } else { " ++ t2.pretty ++ " }"
+  | .Public => "Public"
+  | .Sing b => "Sing(" ++ b.pretty ++ ")"
+  | .default => "default"
+
+instance : ToString (ty l d) where
+  toString := ty.pretty
